wip

extra/SepROExtra.v
@@ -454,3 +454,229 @@ Proof using.
   lets (MP&ME): hpure_inv P1. rewrites (rm ME).
   rewrites~ (>> N P2). rew_fmap~.
 Qed.
+
+
+
+Lemma hstar_hempty_l : forall H,
+  hempty \* H = H.
+Proof using.
+  intros. applys pred_ext_1. intros h.
+  iff (h1&h2&M1&M2&D&U) M.
+  { forwards E: hempty_inv M1. subst.
+    rewrite~ heap_union_empty_l. }
+  { exists~ heap_empty h. }
+Qed.
+
+Lemma hstar_comm : forall H1 H2,
+   H1 \* H2 = H2 \* H1.
+Proof using.
+  intros. unfold hprop, hstar. extens. intros h.
+  hint Fmap.agree_sym.
+  iff (h1&h2&M1&M2&D&U).
+  { exists h2 h1. subst. splits~. }
+  { exists h2 h1. subst. splits~. }
+Qed.
+
+Lemma hstar_assoc : forall H1 H2 H3,
+  (H1 \* H2) \* H3 = H1 \* (H2 \* H3).
+Proof using.
+  intros. unfold hprop, hstar. extens. intros h. split.
+  { intros (h'&h3&(h1&h2&M2&P1&P2&E1)&M3&M1&E2). subst h'.
+    lets~ (M1a&M1b): heap_compat_union_l_inv M1.
+    exists h1 (h2 \u h3). splits.
+    { auto. }
+    { exists h2 h3. splits*. }
+    { applys* heap_compat_union_r. }
+    { subst. applys~ heap_union_assoc. } }
+  { intros (h1&h'&P1&(h2&h3&M2&P2&P3&E1)&M1&E2). subst h'.
+    lets~ (M1a&M1b): heap_compat_union_r_inv M1.
+    exists (h1 \u h2) h3. splits.
+    { exists h1 h2. splits*. }
+    { auto. }
+    { applys* heap_compat_union_l. }
+    { subst. symmetry. applys~ heap_union_assoc. } }
+Qed.
+
+Lemma hstar_hexists : forall A (J:A->hprop) H,
+  (hexists J) \* H = hexists (fun x => (J x) \* H).
+Proof using.
+  intros. applys pred_ext_1. intros h. iff M.
+  { destruct M as (h1&h2&(x&M1)&M2&D&U). exists~ x h1 h2. }
+  { destruct M as (x&(h1&h2&M1&M2&D&U)). exists h1 h2. splits~. exists~ x. }
+Qed.
+
+Lemma hstar_hforall : forall H A (J:A->hprop),
+  (hforall J) \* H ==> hforall (J \*+ H).
+Proof using.
+  intros. intros h M. destruct M as (h1&h2&M1&M2&D&U). intros x. exists~ h1 h2.
+Qed.
+
+Lemma himpl_frame_l : forall H2 H1 H1',
+  H1 ==> H1' ->
+  (H1 \* H2) ==> (H1' \* H2).
+Proof using. introv W (h1&h2&?). exists* h1 h2. Qed.
+
+Lemma haffine_hempty :
+  haffine \[].
+Proof using.
+  introv K. rewrite (hempty_inv K). applys heap_affine_empty.
+Qed.
+
+Lemma haffine_hstar : forall H1 H2,
+  haffine H1 ->
+  haffine H2 ->
+  haffine (H1 \* H2).
+Proof using.
+  introv M1 M2 (h1&h2&K1&K2&D&->). applys* heap_affine_union.
+Qed
+
+
+
+Definition onlyrw (H:hprop) : Prop :=
+  forall h, H h -> h^^ro = Fmap.empty.
+
+Definition onlyrw_post A (Q:A->hprop) : Prop :=
+  forall x, onlyrw (Q x).
+
+Lemma onlyrw_part_ro : forall H h,
+  onlyrw H ->
+  H h ->
+  h^^ro = Fmap.empty.
+Proof using. introv N K. applys* N. Qed.
+
+Lemma onlyrw_part_rw : forall H h,
+  onlyrw H ->
+  H h ->
+  h^^rw = h.
+Proof using.
+  introv N K. specializes N (rm K).
+  rewrite heap_state_def. rewrite N. rew_fmap*.
+Qed.
+
+Lemma onlyrw_proj_ro : forall H h,
+  onlyrw H ->
+  H h ->
+  h^ro = heap_empty.
+Proof using. introv N K. applys heap_eq; simple*. Qed.
+
+Lemma onlyrw_proj_rw : forall H h,
+  onlyrw H ->
+  H h ->
+  h^rw = h.
+Proof using.
+  introv N K.
+  applys heap_eq_projs; rew_heap*.
+  specializes N (rm K).
+
+ applys heap_eq. split*. rew_heap.
+
+  heap_eq_projs
+
+Qed.
+  introv N K. specializes N (rm K).
+  rewrite heap_state_def. rewrite N. rew_fmap*.
+Qed.
+
+Lemma onlyrw_of_haffine : forall H,
+  haffine H ->
+  onlyrw H.
+Proof using.
+  introv M. intros h K. rewrite haffine_eq in M.
+  specializes M K. applys* heap_affine_onlyrw.
+Qed.
+
+Lemma onlyrw_hempty :
+  onlyrw \[].
+Proof using.
+  Transparent hempty hpure.
+  introv M. unfolds hempty, hpure. subst. rew_heap*.
+Qed.
+
+Lemma onlyrw_hpure : forall P,
+  onlyrw \[P].
+Proof using.
+  Transparent hpure.
+  introv (p&M). unfolds hempty. subst. rew_heap*.
+Qed.
+
+Lemma onlyrw_hgc :
+  onlyrw \GC.
+Proof using.
+  introv (H&M). rewrite hstar_hpure_l in M. destruct M as (F&R).
+  applys* heap_affine_onlyrw. rewrite haffine_eq in F. applys* F.
+Qed.
+
+Lemma onlyrw_hempty' : (* simpler proof *)
+  onlyrw \[].
+Proof using.
+  intros. rewrite hempty_eq_hpure_true. applys~ onlyrw_hpure.
+Qed.
+
+Lemma onlyrw_hsingle : forall l v,
+  onlyrw (hsingle l v).
+Proof using. introv (E&N). autos*. Qed.
+
+Lemma onlyrw_hstar : forall H1 H2,
+  onlyrw H1 ->
+  onlyrw H2 ->
+  onlyrw (H1 \* H2).
+Proof using.
+  introv N1 N2 (h1&h2&P1&P2&M1&->). rew_heap*.
+  rewrites (>> N1 P1). rewrites (>> N2 P2). rew_fmap*.
+Qed.
+
+Lemma onlyrw_hexists : forall A (J:A->hprop),
+  onlyrw_post J ->
+  onlyrw (hexists J).
+Proof using. introv M (x&N). rewrites~ (>> M N). Qed.
+
+Hint Resolve onlyrw_hempty onlyrw_hstar onlyrw_hgc : onlyrw.
+
+(* Remaining lemmas are not needed for the soundness proof,
+   but may be needed by clients. *)
+
+Lemma onlyrw_hforall_inhab : forall `{Inhab A} (J:A->hprop),
+  onlyrw_post J ->
+  onlyrw (hforall J).
+Proof using.
+  introv IA M N. lets M': M (arbitrary (A:=A)). lets N': N (arbitrary (A:=A)).
+  applys M' N'.
+Qed.
+
+Lemma onlyrw_hforall : forall A (x:A) (J:A->hprop),
+  onlyrw (J x) ->
+  onlyrw (hforall J).
+Proof using. introv M N. applys M N. Qed.
+
+Lemma onlyrw_hor : forall H1 H2,
+  onlyrw H1 ->
+  onlyrw H2 ->
+  onlyrw (hor H1 H2).
+Proof using. introv M1 M2. applys onlyrw_hexists. intros b. case_if*. Qed.
+
+Lemma onlyrw_hand_l : forall H1 H2,
+  onlyrw H1 ->
+  onlyrw (hand H1 H2).
+Proof using. introv M1. applys* onlyrw_hforall true. Qed.
+
+Lemma onlyrw_hand_r : forall H1 H2,
+  onlyrw H2 ->
+  onlyrw (hand H1 H2).
+Proof using. introv M1. applys* onlyrw_hforall false. Qed.
+
+Lemma onlyrw_himpl : forall H1 H2,
+  onlyrw H2 ->
+  (H1 ==> H2) ->
+  onlyrw H1.
+Proof using. introv HS HI M. lets: HI M. applys* HS. Qed.
+
+(* Note: onlyrw_hwand is not true *)
+
+Lemma onlyrw_hpure_star_hpure : forall (P:Prop) H,
+  (P -> onlyrw H) ->
+  onlyrw (\[P] \* H).
+Proof using.
+  introv N (h1&h2&P1&P2&M1&->). rew_heap*.
+  lets (MP&ME): hpure_inv P1. rewrites (rm ME).
+  rew_fmap. rewrites~ (>> N P2).
+Qed.
